theories/Eq.v
@@ -1,0 +1,50 @@
+From Coinduction Require Export
+     coinduction rel tactics.
+
+From CTree Require Import CTrees.
+From CTree.Eq Require Export
+     Equ
+     Trans
+     SBisim.
+
+Export CTreeNotations.
+Export EquNotations.
+Export SBisimNotations.
+
+#[global] Tactic Notation "step" :=
+  __step_equ || __step_sbisim.
+
+#[global] Tactic Notation "coinduction" simple_intropattern(R) simple_intropattern(H) :=
+  __coinduction_equ R H || __coinduction_sbisim R H.
+
+#[global] Tactic Notation "step" "in" ident(H) :=
+  __step_in_equ H || __step_in_sbisim H.
+
+#[global] Tactic Notation "upto_vis" := __upto_vis_sbisim.
+
+#[global] Tactic Notation "play" := __play_sbisim.
+#[global] Tactic Notation "playL" "in" ident(H) := __playL_sbisim H.
+#[global] Tactic Notation "playR" "in" ident(H) := __playR_sbisim H.
+#[global] Tactic Notation "eplayL" := __eplayL_sbisim.
+#[global] Tactic Notation "eplayR" := __eplayR_sbisim.
+
+#[global] Tactic Notation "upto_bind" :=
+  __eupto_bind_equ || __upto_bind_sbisim.
+
+#[global] Tactic Notation "upto_bind_eq" :=
+  __upto_bind_eq_equ || __upto_bind_eq_sbisim.
+
+#[global] Tactic Notation "upto_bind" "with" uconstr(SS) :=
+  __upto_bind_equ SS.
+
+Ltac eq2equ H :=
+  match type of H with
+  | ?u = ?t => let eq := fresh "EQ" in assert (eq : u ≅ t) by (subst; reflexivity); clear H
+  end.
+
+Ltac eq2sb H :=
+  match type of H with
+  | ?u = ?t => let eq := fresh "EQ" in assert (eq : u ~ t) by (subst; reflexivity); clear H
+  end.
+
+#[global] Opaque wtrans.
