theories/Eq/WBisim.v
@@ -1,0 +1,780 @@
+(*|
+=========================================
+Strong and Weak Bisimulations over ctrees
+=========================================
+The [equ] relation provides [ctree]s with a suitable notion of equality.
+It is however much too fine to properly capture any notion of behavioral
+equivalence that we could want to capture over computations modelled as
+[ctree]s.
+If we draw a parallel with [itree]s, [equ] maps directly to [eq_itree],
+while [eutt] was introduced to characterize computations that exhibit the
+same external observations, but may disagree finitely on the amount of
+internal steps occuring between any two observations.
+While the only consideration over [itree]s was to be insensitive to the
+amount of fuel needed to run, things are richer over [ctree]s.
+We essentially want to capture three intuitive things:
+- to be insensitive to the particular branches chosen at non-deterministic
+nodes -- in particular, we want [choice t u ~~ choice u t];
+- to always be insensitive to how many _invisible_ choice nodes are crawled
+through -- they really are a generalization of [Tau] in [itree]s;
+- to have the flexibility to be sensible or not to the amount of _visible_
+choice nodes encountered -- they really are a generalization of CCS's tau
+steps. This last fact, whether we observe or not these nodes, will constrain
+the distinction between the weak and strong bisimulations we define.
+
+In contrast with [equ], as well as the relations in [itree]s, we do not
+define the functions generating the relations directly structurally on
+the trees. Instead, we follow a definition closely following the style
+developed for process calculi, essentially stating that diagrams of this
+shape can be closed.
+t  R  u
+|     |
+l     l
+v     v
+t' R  u'
+The transition relations that we use to this end are defined in the [Trans]
+module:
+- strong bisimulation is defined as a symmetric games over [trans];
+- weak bisimulation is defined as an asymmetric game in which [trans] get
+answered by [wtrans].
+
+.. coq::none
+|*)
+From Coinduction Require Import
+     coinduction rel tactics.
+
+From CTree Require Import
+     Utils CTrees Eq.Equ Shallow Eq.Trans Eq.SBisim.
+
+From RelationAlgebra Require Import
+     monoid
+     kat
+     kat_tac
+     prop
+     rel
+     srel
+     comparisons
+     rewriting
+     normalisation.
+
+Import CTree.
+Import CTreeNotations.
+Import EquNotations.
+Import SBisimNotations.
+
+(*|
+Weak Bisimulation
+-------------------
+Relation relaxing [equ] to become insensible to:
+- the amount of (any kind of) choices taken;
+- the particular branches taken during (any kind of) choices.
+|*)
+
+Section WeakBisim.
+
+  Context {E : Type -> Type} {X : Type}.
+  Notation S := (ctree E X).
+
+(*|
+The function defining weak simulations: [trans] plays must be answered
+using [wtrans].
+The [ws] definition stands for [weak simulation]. The bisimulation [wb]
+is once again obtained by expliciting the symmetric aspect of the definition.
+|*)
+  Program Definition ws: mon (rel S S) :=
+    {| body R p q :=
+      forall l p', trans l p p' -> exists2 q', wtrans l q q' & R p' q' |}.
+  Next Obligation. destruct (H0 _ _ H1). eauto. Qed.
+
+(*|
+The bisimulation is obtained by intersecting [ws] with its symmetrized version.
+|*)
+  Definition wb := (Coinduction.lattice.cap ws (comp converse (comp ws converse))).
+
+(*|
+The function defining one-sided expansion (standard notion in process algebra).
+This relation echoes [euttge] over [itrees]: the amount of fuel required on either
+side of the computation can only decrease from left to right, not the other way around.
+We are not interested in this relation by itself, but it is an important proof intermediate.
+|*)
+  Program Definition es: mon (rel S S) :=
+    {| body R p q :=
+      forall l p', trans l p p' -> exists2 q', etrans l q q' & R p' q' |}.
+  Next Obligation. destruct (H0 _ _ H1). eauto. Qed.
+
+End WeakBisim.
+
+(*|
+The relation itself
+|*)
+Definition wbisim {E X} := (gfp (@wb E X): hrel _ _).
+
+Module WBisimNotations.
+
+  Notation "p ≈ q" := (wbisim p q) (at level 70).
+  Notation wt := (coinduction.t wb).
+  Notation wT := (coinduction.T wb).
+  Notation wbt := (coinduction.bt wb).
+  Notation wbT := (coinduction.bT wb).
+(*|
+Notations  for easing readability in proofs by enhanced coinduction
+|*)
+  Notation "x [≈] y" := (wt _ x y) (at level 80).
+  Notation "x {≈} y" := (wbt _ x y) (at level 80).
+  Notation "t {{≈}} u" := (wb _ t u) (at level 79).
+
+End WBisimNotations.
+
+Import WBisimNotations.
+
+Ltac fold_wbisim :=
+  repeat
+    match goal with
+    | h: context[@wb ?E ?X] |- _ => fold (@wbisim E X) in h
+    | |- context[@wb ?E ?X]      => fold (@wbisim E X)
+    end.
+
+Ltac __coinduction_wbisim R H :=
+  unfold wbisim; apply_coinduction; fold_wbisim; intros R H.
+
+Tactic Notation "__step_wbisim" :=
+  match goal with
+  | |- context[@wbisim ?E ?X] =>
+      unfold wbisim;
+      step;
+      fold (@wbisim E X)
+  | |- _ => step
+  end.
+
+#[local] Tactic Notation "step" := __step_wbisim.
+
+#[local] Tactic Notation "coinduction" simple_intropattern(R) simple_intropattern(H) :=
+  __coinduction_wbisim R H.
+
+Ltac __step_in_wbisim H :=
+  match type of H with
+  | context [@wbisim ?E ?X] =>
+      unfold wbisim in H;
+      step in H;
+      fold (@wbisim E X) in H
+  end.
+
+#[local] Tactic Notation "step" "in" ident(H) := __step_in_wbisim H.
+
+Ltac twplayL_ tac :=
+  match goal with
+  | h : @wbisim ?E ?X _ _ |- _ =>
+      step in h;
+      let Hf := fresh "Hf" in
+      destruct h as [Hf _];
+      cbn in Hf; edestruct Hf as [? ?TR ?EQ];
+      [tac | clear Hf]
+  end.
+
+Tactic Notation "twplayL" tactic(t) := twplayL_ t.
+Ltac wplayL H := twplayL ltac:(apply @H).
+Ltac ewplayL := twplayL etrans.
+
+Ltac twplayR_ tac :=
+  match goal with
+  | h : @wbisim ?E ?X _ _ |- _ =>
+      step in h;
+      let Hb := fresh "Hb" in
+      destruct h as [_ Hb];
+      cbn in Hb; edestruct Hb as [? ?TR ?EQ];
+      [tac | clear Hb]
+  end.
+
+Tactic Notation "twplayR" tactic(t) := twplayR_ t.
+Ltac wplayR H := twplayR ltac:(apply @H).
+Ltac ewplayR := twplayR etrans.
+
+Section wbisim_theory.
+
+	Context {E : Type -> Type} {X : Type}.
+  Notation ws := (@ws E X).
+  Notation wb := (@wb E X).
+  Notation wbisim  := (@wbisim E X).
+  Notation wt  := (coinduction.t wb).
+  Notation wbt := (coinduction.bt wb).
+  Notation wT  := (coinduction.T wb).
+
+(*|
+Elementary properties of [wbisim]
+----------------------------------------------
+We have in short:
+- [ss ≤ es ≤ ws] (direct consequence of transition relations' properties)
+- [sbisim] ⊆ [wbisim]
+- [equ] ⊆ [wbisim]
+- [wbisim] is closed under [equ]
+- [wbisim] is closed under [bisim]
+- up-to reflexivity
+- up-to symmetry
+- transitivity (but NOT up-to transitivity)
+
+We naturally also have [equ] ⊆ [sbisim], and hence [equ] ⊆  [wbisim], but we need
+to work a bit more to establish it.
+It is a consequence more generally of [sbisim] and [wbisim] being closed under [equ]
+on both arguments.
+We also get [wbisim] closed under [sbism] on both arguments, but need first to
+establish [wbisim]'s transitivity for that.
+|*)
+    Lemma s_e: @ss E X <= es.
+    Proof. intros R p q H l p' pp'. destruct (H _ _ pp'). eauto using trans_etrans_. Qed.
+    Lemma e_w: es <= ws.
+    Proof. intros R p q H l p' pp'. destruct (H _ _ pp'). eauto using etrans_wtrans_. Qed.
+    Lemma s_w: ss <= ws.
+    Proof. rewrite s_e. apply e_w. Qed.
+
+    Corollary sbisim_wbisim: sbisim <= wbisim.
+    Proof.
+      apply gfp_leq.
+      apply Coinduction.lattice.cap_leq. apply s_w.
+      intros R p q. apply (@s_w (R°) q p).
+    Qed.
+
+    #[global] Instance sbisim_wbisim_subrelation : subrelation sbisim wbisim.
+    Proof.
+      apply sbisim_wbisim.
+    Qed.
+
+(*|
+Since [wt R] contains [wbisim] that contains [sbisim] which is known to be reflexive,
+it is reflexive as well
+|*)
+    #[global] Instance Reflexive_wt R: Reflexive (wt R).
+    Proof. intro. apply (gfp_t wb). now apply sbisim_wbisim. Qed.
+
+(*|
+[converse] is compatible
+|*)
+    Lemma converse_wt: converse <= wt.
+    Proof. apply invol_t. Qed.
+
+(*|
+Hence [wt R] is always symmetric
+|*)
+    #[global] Instance Symmetric_wt R: Symmetric (wt R).
+    Proof. intros ??. apply (ft_t converse_wt). Qed.
+
+(*|
+[wbism] is closed under [equ]
+|*)
+    #[global] Instance equ_wbisim_compat_goal : Proper (equ eq ==> equ eq ==> flip impl) wbisim.
+    Proof.
+      intros t t' eqt u u' equ; cbn.
+      revert t t' u u' eqt equ.
+      unfold wbisim; coinduction ? CIH; fold wbisim in *.
+      intros * eqt equ eqtu.
+      step in eqtu.
+      destruct eqtu as [ftu btu].
+      split.
+      + intros ? ? ?.
+        rewrite eqt in H.
+        apply ftu in H as [?u' T eq].
+        eexists. rewrite equ. apply T.
+        eapply CIH; try reflexivity; auto.
+      + intros ? ? ?.
+        rewrite equ in H.
+        apply btu in H as [?t' T eq].
+        eexists. rewrite eqt. apply T.
+        eapply CIH; try reflexivity; auto.
+    Qed.
+
+    #[global] Instance equ_wbisim_compat_ctx : Proper (equ eq ==> equ eq ==> impl) wbisim.
+    Proof.
+      intros t t' eqt u u' equ; cbn.
+      revert t t' u u' eqt equ.
+      unfold wbisim; coinduction ? CIH; fold wbisim in *.
+      intros * eqt equ eqtu.
+      step in eqtu.
+      destruct eqtu as [ftu btu].
+      split.
+      + intros ? ? ?.
+        rewrite <- eqt in H.
+        apply ftu in H as [?u' T eq].
+        eexists. rewrite <- equ. apply T.
+        eapply CIH; try reflexivity; auto.
+      + intros ? ? ?.
+        rewrite <- equ in H.
+        apply btu in H as [?t' T eq].
+        eexists. rewrite <- eqt. apply T.
+        eapply CIH; try reflexivity; auto.
+    Qed.
+
+(*|
+Hence [equ eq] is a included in [wbisim]
+|*)
+    #[global] Instance equ_wbisim_subrelation : subrelation (equ eq) wbisim.
+    Proof.
+      red; intros.
+      rewrite H; reflexivity.
+    Qed.
+
+(*|
+Transitivity
+~~~~~~~~~~~~
+As for weak bisimulation on process algebra, [square] is not a valid
+enhancing function (an explicit counter example is provided below,
+see [not_square_wt]).
+Weak bisimilariy is however transitive nonetheless. We can actually
+reproduce directly Pous' proof for CCS, the relation between [trans] and [wtrans]
+being exactly the same in both cases, even if the underlying objects
+and transitions are completely different.
+|*)
+
+(*|
+Moving to the [srel] world once again to establish algebaric laws based
+on operators from the relation algebra library.
+|*)
+    #[local] Instance equ_wbisim_compat : Proper (equ eq ==> equ eq ==> iff) wbisim.
+    Proof.
+      split; intros.
+      now rewrite <- H, <- H0.
+      now rewrite H, H0.
+    Qed.
+
+    Definition wbisimT : srel SS SS :=
+      {| hrel_of := wbisim : hrel SS SS |}.
+
+(*|
+Algebraic reformulation of the right-to-left part of the game
+
+Note: We can express these laws in the setoid world or not.
+Unclear if there's a benefit to either at this point, we do everything
+on the setoid side.
+|*)
+    Lemma wbisim_trans_back l: wbisimT ⋅ trans l ≦ wtrans l ⋅ wbisimT.
+    Proof.
+      intros p q' [q pq qq']. apply (gfp_pfp wb) in pq as [_ pq]. now apply pq.
+    Qed.
+    Lemma wbisim_trans_back' l: wbisim ⋅ transR l ≦ (wtrans l : hrel _ _) ⋅ wbisim.
+    Proof.
+      intros p q' [q pq qq']. apply (gfp_pfp wb) in pq as [_ pq]. now apply pq.
+    Qed.
+    Lemma wbisim_etrans_back l: wbisimT ⋅ etrans l ≦ wtrans l ⋅ wbisimT.
+    Proof.
+      unfold etrans; destruct l.
+      2,3: apply @wbisim_trans_back.
+      ra_normalise. rewrite wbisim_trans_back.
+      unfold wtrans, etrans. ka.
+    Qed.
+    Lemma wbisim_taus_back: wbisimT ⋅ (trans tau)^* ≦ (trans tau)^* ⋅ wbisimT.
+    Proof.
+      rewrite <-str_invol at 2.
+      apply str_move_l. rewrite wbisim_trans_back. unfold wtrans, etrans. ka.
+    Qed.
+    Lemma wbisim_wtrans_back l: wbisimT ⋅ wtrans l ≦ wtrans l ⋅ wbisimT.
+    Proof.
+      unfold wtrans.
+      mrewrite wbisim_taus_back.
+      mrewrite wbisim_etrans_back.
+      mrewrite wbisim_taus_back.
+      unfold wtrans, etrans. ka.
+    Qed.
+
+    Lemma cnv_wt R: (wt R: hrel _ _)° ≡ wt R.
+    Proof. apply RelationAlgebra.lattice.antisym; intros ???; now apply Symmetric_wt. Qed.
+    Lemma cnv_gfp: RelationAlgebra.lattice.weq ((gfp wb: hrel _ _)°) (gfp wb).
+    Proof. apply cnv_wt. Qed.
+    Lemma cnv_wbisim: wbisimT° ≡ wbisimT.
+    Proof. apply cnv_wt. Qed.
+    Lemma cnv_wbisim': wbisim° ≡ wbisim.
+    Proof. apply cnv_wt. Qed.
+
+
+(*|
+By symmetry, similar results for left-to-right game
+|*)
+    Lemma wbisim_trans_front l: (trans l)° ⋅ wbisimT ≦ wbisimT ⋅ (wtrans l)°.
+    Proof. cnv_switch. rewrite 2cnvdot, cnv_invol, cnv_wbisim. apply wbisim_trans_back. Qed.
+    Lemma wbisim_etrans_front l: (etrans l)° ⋅ wbisimT ≦ wbisimT ⋅ (wtrans l)°.
+    Proof. cnv_switch. rewrite 2cnvdot, cnv_invol, cnv_wbisim. apply wbisim_etrans_back. Qed.
+    Lemma wbisim_wtrans_front l: (wtrans l)° ⋅ wbisimT ≦ wbisimT ⋅ (wtrans l)°.
+    Proof. cnv_switch. rewrite 2cnvdot, cnv_invol, cnv_wbisim. apply wbisim_wtrans_back. Qed.
+
+(*|
+Explicit, non-algebraic version
+|*)
+    Lemma wbisim_wtrans_front_ p q l p': wtrans l p p' -> p ≈ q -> exists2 q', p' ≈ q' & @wtrans E X l q q'.
+    Proof. intros pp' pq. apply wbisim_wtrans_front. now exists p. Qed.
+
+(*|
+Finally, the proof of transitivity
+|*)
+    #[global] Instance Transitive_wbisim: Transitive wbisim.
+    Proof.
+      assert (square wbisim <= wbisim) as H.
+      apply leq_gfp. apply symmetric_pfp.
+      rewrite converse_square.
+      apply square. simpl. apply cnv_gfp.
+      intros x z [y xy yz] l x' xx'.
+      apply (gfp_pfp wb) in xy as [xy _].
+      destruct (xy _ _ xx') as [y' yy' x'y'].
+      destruct (wbisim_wtrans_front_ _ _ _ _ yy' yz) as [z' y'z' zz'].
+      exists z'. assumption. now exists y'.
+      intros x y z xy yz. apply H. now exists y.
+    Qed.
+
+    #[global] Instance Equivalence_wbisim: Equivalence wbisim.
+    Proof.
+      split; typeclasses eauto.
+    Qed.
+
+(*|
+We can now easily derive that [wbisim] is closed under [sbisim]
+|*)
+    #[global] Instance sbisim_wbisim_closed_goal : Proper (sbisim ==> sbisim ==> flip impl) wbisim.
+    Proof.
+      repeat intro.
+      now rewrite H, H0.
+    Qed.
+
+    #[global] Instance sbisim_wbisim_closed_ctx : Proper (sbisim ==> sbisim ==> impl) wbisim.
+    Proof.
+      repeat intro.
+      now rewrite <- H, <- H0.
+    Qed.
+
+#[global] Opaque wtrans.
+
+(*|
+Weak bisimulation up-to [equ] is valid
+|*)
+    Lemma equ_clos_wt : @equ_clos E X X <= wt.
+    Proof.
+      apply Coinduction, by_Symmetry; [apply equ_clos_sym |].
+      intros R t u EQ l t1 TR; inv EQ.
+      destruct HR as [F _]; cbn in *.
+      rewrite Equt in TR.
+      apply F in TR.
+      destruct TR as [? ? ?].
+      eexists.
+      rewrite <- Equu; eauto.
+      apply (f_Tf wb).
+      econstructor; intuition.
+      auto.
+    Qed.
+
+(*|
+We can therefore rewrite [equ] in the middle of bisimulation proofs
+|*)
+    #[global] Instance equ_clos_wt_proper_goal RR :
+      Proper (equ eq ==> equ eq ==> flip impl) (wt RR).
+    Proof.
+      cbn; unfold Proper, respectful; intros.
+      apply (ft_t equ_clos_wt).
+      econstructor; [eauto | | symmetry; eauto]; auto.
+    Qed.
+
+    #[global] Instance equ_clos_wt_proper_ctx RR :
+      Proper (equ eq ==> equ eq ==> impl) (wt RR).
+    Proof.
+      cbn; unfold Proper, respectful; intros.
+      apply (ft_t equ_clos_wt).
+      econstructor; [symmetry; eauto | | eauto]; auto.
+    Qed.
+
+(*|
+Contrary to what happens with [sbisim], weak bisimulation ignores both kinds of taus
+|*)
+
+    Lemma tauI_wb : forall (t : ctree E X),
+        TauI t ≈ t.
+    Proof.
+      intros. now rewrite sb_tauI.
+    Qed.
+
+    Lemma tauV_wb : forall (t : ctree E X),
+        TauV t ≈ t.
+    Proof.
+      intros t; step; split.
+      - intros l t' H.
+        apply trans_tauV_inv in H as [EQ ->].
+        exists t'.
+        rewrite EQ. apply wnil.
+        reflexivity.
+      - intros l t' H. exists t'.
+        apply wtrans_tauV.
+        apply trans_wtrans; auto.
+        cbn; reflexivity.
+    Qed.
+
+(*|
+Disproving the transitivity of [wt R]
+-------------------------------------
+|*)
+
+    Lemma not_Transitive_wt Z: X -> Z -> E Z -> ~ forall R, Transitive (wt R).
+    Proof.
+      intros x z e H.
+      cut (Vis e (fun _ => Ret x) ≈ Ret x).
+      - intros abs. step in abs; destruct abs as [abs _].
+        destruct (abs (obs e z) (Ret x)) as [? step EQ].
+        constructor; reflexivity.
+        apply wtrans_ret_inv in step as [[abs' ?] | [abs' ?]]; inv abs'.
+      - rewrite <- tauV_wb.
+        rewrite <- (tauV_wb (Ret x)).
+        unfold wbisim; coinduction ? CIH; fold wbisim in *.
+        split.
+        + intros l t' tt'.
+          apply trans_tauV_inv in tt' as [EQ ->].
+          exists (Ret x); auto.
+          apply trans_wtrans; constructor; [exact Fin.F1 | reflexivity].
+          apply equ_wbisim_subrelation in EQ.
+          rewrite EQ.
+          rewrite <- (subrelation_gfp_t _ (tauV_wb _)).
+          rewrite <- (subrelation_gfp_t _ (tauV_wb (Ret x))).
+          assumption.  (* Here clearly some instances are missing, the rewrite do not work in the other order, and should not require such an explicit low level call *)
+        + intros ? ? ?.
+          apply trans_tauV_inv in H0 as [EQ ->].
+          eexists.
+          apply trans_wtrans; constructor; [exact Fin.F1 | reflexivity].
+          cbn.
+          apply equ_wbisim_subrelation in EQ.
+          rewrite <- (subrelation_gfp_t _ (tauV_wb _)).
+          symmetry.
+          rewrite EQ.
+          rewrite <- (subrelation_gfp_t _ (tauV_wb _)).
+          symmetry.
+          assumption.
+    Qed.
+
+    Lemma not_square_wt Z: X -> Z -> E Z -> ~ square <= wt.
+    Proof.
+      intros x z e H. elim (not_Transitive_wt _ x z e). intro R.
+      intros ? y ???. apply (ft_t H). now exists y.
+    Qed.
+
+End wbisim_theory.
+
+Section bind.
+
+  Obligation Tactic := idtac.
+  Context {E : Type -> Type} {X Y: Type}.
+
+(*|
+Specialization of [bind_ctx] to a function acting with [sbisim] on the bound value,
+and with the argument (pointwise) on the continuation.
+|*)
+  Program Definition bind_ctx_wbisim :  mon (rel (ctree E Y) (ctree E Y)) :=
+    {|body := fun R => @bind_ctx E X X Y Y wbisim (pointwise eq R) |}.
+  Next Obligation.
+    intros ???? H. apply leq_bind_ctx. intros ?? H' ?? H''.
+    apply in_bind_ctx. apply H'. intros t t' HS. apply H0, H'', HS.
+  Qed.
+
+(*|
+Sufficient condition to exploit symmetry
+|*)
+    Lemma bind_ctx_wbisim_sym: compat converse bind_ctx_wbisim.
+    Proof.
+      intro R. simpl. apply leq_bind_ctx. intros. apply in_bind_ctx.
+      symmetry; auto.
+      intros ? ? ->.
+      apply H0; auto.
+    Qed.
+
+(*|
+The resulting enhancing function gives a valid up-to technique
+|*)
+    Lemma bind_ctx_wbisim_t : bind_ctx_wbisim <= wt.
+    Proof.
+      apply Coinduction, by_Symmetry.
+      apply bind_ctx_wbisim_sym.
+      intros R. apply (leq_bind_ctx _).
+      intros t1 t2 tt k1 k2 kk.
+      step in tt; destruct tt as (F & B); cbn in *.
+      cbn in *; intros l u STEP.
+      apply trans_bind_inv in STEP as [(H & t' & STEP & EQ) | (v & STEPres & STEP)]; cbn in *.
+      - apply F in STEP as [u' STEP EQ'].
+        eexists.
+        apply wtrans_bind_l; eauto.
+        apply (fT_T equ_clos_wt).
+        econstructor; [exact EQ | | reflexivity].
+        apply (fTf_Tf wb).
+        apply in_bind_ctx; auto.
+        intros ? ? ->.
+        apply (b_T wb).
+        apply kk; auto.
+      - clear B.
+        (* Things are tricky, the bind inversion rule is messy *)
+        specialize (kk v v eq_refl).
+        destruct kk as [F' _].
+        apply F  in STEPres as [x STEPres EQ].
+        apply F' in STEP    as [u' STEP HR].
+        pose proof (wtrans_val_inv' STEPres) as (? & wtr & ? & EQ').
+        rewrite EQ' in STEPres.
+        pose proof wtrans_bind_r _ STEPres STEP as [EQ'' | ?].
+        + rewrite EQ'' in STEP.
+          assert (l = tau) by admit.
+          subst.
+          exists (k2 v).
+          admit.
+          admit.
+        + admit.
+
+    Admitted.
+
+End bind.
+
+(*|
+Expliciting the reasoning rule provided by the up-to principles.
+|*)
+Lemma wbisim_clo_bind (E: Type -> Type) (X Y : Type) :
+	forall (t1 t2 : ctree E X) (k1 k2 : X -> ctree E Y) RR,
+		t1 ≈ t2 ->
+    (forall x, (wt RR) (k1 x) (k2 x)) ->
+    wt RR (t1 >>= k1) (t2 >>= k2)
+.
+Proof.
+  intros.
+  apply (ft_t (@bind_ctx_wbisim_t E X Y)).
+  apply in_bind_ctx; auto.
+  intros ? ? <-; auto.
+Qed.
+
+(*|
+And in particular, we get the proper instance justifying rewriting [~]
+and [≈] to the left of a [bind].
+|*)
+#[global] Instance bind_wbisim_cong :
+ forall (E : Type -> Type) (X Y : Type) (R : rel Y Y) RR,
+   Proper (wbisim ==> pointwise_relation X (wt RR) ==> wt RR) (@bind E X Y).
+Proof.
+  repeat red; intros; eapply wbisim_clo_bind; eauto.
+Qed.
+
+Lemma wbisim_ret_inv {E R} : forall (x y : R),
+    Ret x ≈ (Ret y : ctree E R) ->
+    x = y.
+Proof.
+  intros * EQ.
+  ewplayL.
+  apply wtrans_case' in TR as [(?v & TR & WTR)|(?v & TR & WTR)].
+  inv_trans; auto.
+  inv_trans; auto.
+Qed.
+
+(*|
+Note: with choiceI2, these relations hold up-to strong bisimulation.
+With choiceV2 however they don't even hold up-to weak bisimulation.
+|*)
+Lemma spinV_nary_0 : forall {E R}, @spinV_nary E R 0 ≈ spinV_nary 0.
+Proof.
+  intros E R.
+  reflexivity.
+Qed.
+
+Ltac wcase :=
+  match goal with
+    [ h   : hrel_of (wtrans ?l) _ _,
+      bis : wbisim _ _
+      |- _] =>
+      let EQ := fresh "EQ" in
+      match l with
+      | tau => apply wtrans_case' in h as [EQ|(? & ?TR & ?WTR)];
+              [rewrite <- EQ in bis; clear EQ |]
+      | _   => apply wtrans_case' in h as [(? & ?TR & ?WTR)|(? & ?TR & ?WTR)]
+      end
+  end.
+
+#[local] Arguments trans_choiceV21 [_ _].
+#[local] Arguments trans_choiceV22 [_ _].
+#[local] Arguments trans_ret [_ _] _.
+
+(*|
+With choiceV2 however they don't even hold up-to weak bisimulation.
+The proof is not interesting, but it would be good to have a
+light way to automate it, so it's a decent case study.
+|*)
+Lemma choiceV2_not_assoc :
+	~ (choiceV2 (choiceV2 (Ret 0 : ctree Sum.void1 nat) (Ret 1)) (Ret 2) ≈ choiceV2 (Ret 0) (choiceV2 (Ret 1) (Ret 2)))%nat.
+Proof.
+  intros abs.
+
+  (* init: 012 || 012 *)
+  wplayL trans_choiceV21.
+
+  (* PL  : 01  || 012 *)
+  wcase.
+  - (* AR:  01  || 012 *)
+    wplayR trans_choiceV22.
+    (* PR:  01  ||  12 *)
+    wcase.
+    + (* AL:  01  ||  12 *)
+      wplayR trans_choiceV22.
+      (* PR:  01  ||   2 *)
+      wcase.
+      * (* AL: 01  ||   2 *)
+        wplayR trans_ret.
+        (* PR: 01  |2?|   ∅ *)
+        wcase.
+        (* AL: steps with 2, abs *)
+        inv_trans.
+        inv_trans.
+        (* PR: 0   ||   ∅ *)
+        wcase; inv_trans.
+        (* PR: 1   ||   ∅ *)
+        wcase; inv_trans.
+      * inv_trans.
+        (* AL: 0  ||   2 *)
+        wcase.
+        apply wbisim_ret_inv in EQ; inv EQ.
+        inv_trans.
+        (* AL: 1  ||   2 *)
+        wcase.
+        apply wbisim_ret_inv in EQ; inv EQ.
+        inv_trans.
+    + inv_trans.
+      * (* AL:  0  ||  12 *)
+        wcase.
+        wplayL trans_ret.
+        wcase; inv_trans.
+        wcase; inv_trans.
+        wcase; inv_trans.
+        inv_trans.
+      * (* AL:  1  ||  12 *)
+        wcase.
+        wplayR trans_choiceV22.
+        wcase.
+        apply wbisim_ret_inv in EQ; inv EQ.
+        inv_trans.
+        inv_trans.
+  - inv_trans.
+    + wcase.
+      * wplayL trans_choiceV22.
+        wcase.
+        apply wbisim_ret_inv in EQ; inv EQ.
+        inv_trans.
+      * inv_trans.
+    + wcase.
+      wplayL trans_choiceV21.
+      wcase.
+      wplayL trans_ret.
+      wcase.
+      inv_trans.
+      inv_trans.
+      wcase; inv_trans.
+      wcase; inv_trans.
+      inv_trans.
+      wcase.
+      apply wbisim_ret_inv in EQ; inv EQ.
+      inv_trans.
+      wcase.
+      apply wbisim_ret_inv in EQ; inv EQ.
+      inv_trans.
+      inv_trans.
+      wcase.
+      wplayL trans_choiceV21.
+      wcase.
+      apply wbisim_ret_inv in EQ; inv EQ.
+      inv_trans.
+      inv_trans.
+      wcase.
+      wplayL trans_choiceV21.
+      wcase.
+      apply wbisim_ret_inv in EQ; inv EQ.
+      inv_trans.
+      inv_trans.
+Qed.
